thys/DataRefinementIBP/Statements.thy
@@ -22,18 +22,18 @@ text {*
 
 
 
-lemma mono_top[simp]: "mono top";
-  by (simp add: mono_def top_fun_eq);
+lemma mono_top[simp]: "mono top"
+  by (simp add: mono_def top_fun_eq)
 
 
 
-lemma mono_choice[simp]: "mono S \<Longrightarrow> mono T \<Longrightarrow> mono (S \<sqinter> T)";
-  apply (simp add: mono_def inf_fun_eq);
-  apply safe;
-  apply (rule_tac y = "S x" in order_trans);
-  apply simp_all;
-  apply (rule_tac y = "T x" in order_trans);
-  by simp_all;
+lemma mono_choice[simp]: "mono S \<Longrightarrow> mono T \<Longrightarrow> mono (S \<sqinter> T)"
+  apply (simp add: mono_def inf_fun_eq)
+  apply safe
+  apply (rule_tac y = "S x" in order_trans)
+  apply simp_all
+  apply (rule_tac y = "T x" in order_trans)
+  by simp_all
 
 subsection "Assert statement"
 
@@ -43,7 +43,7 @@ if $s\not\in p$ and behaves as skip otherwise.
 *}
 
 definition
-  "assert p q = p \<sqinter> q";
+  "assert p q = p \<sqinter> q"
 
 subsection "Assume statement"
 
@@ -53,13 +53,13 @@ if $s\not\in p$ and behaves as skip otherwise.
 *}
 
 definition
-  "assume (P::'a::boolean_algebra) Q \<equiv>  -P \<squnion> Q";
+  "assume (P::'a::boolean_algebra) Q \<equiv>  -P \<squnion> Q"
 
-lemma mono_assume [simp]: "mono (assume P)";
-  apply (simp add: assume_def mono_def);
-  apply safe;
+lemma mono_assume [simp]: "mono (assume P)"
+  apply (simp add: assume_def mono_def)
+  apply safe
   apply (rule_tac y = "y" in order_trans)
-  by simp_all;
+  by simp_all
 
 subsection "Demonic update statement"
 
@@ -73,26 +73,26 @@ in $s$.
 *}
 
 definition
-  "demonic Q p = {s . Q s \<le> p}";
+  "demonic Q p = {s . Q s \<le> p}"
 
-lemma mono_demonic [simp]: "mono (demonic Q)";
-  apply (simp add: mono_def demonic_def le_bool_def);
-  by auto;
+lemma mono_demonic [simp]: "mono (demonic Q)"
+  apply (simp add: mono_def demonic_def le_bool_def)
+  by auto
 
 theorem demonic_bottom:
-  "demonic R (\<bottom>::('a::{order, bot})) = {s . (R s) = \<bottom>}";
-  apply (unfold demonic_def);
-  apply auto;
-  apply (rule antisym);
-  by auto;
+  "demonic R (\<bottom>::('a::{order, bot})) = {s . (R s) = \<bottom>}"
+  apply (unfold demonic_def)
+  apply auto
+  apply (rule antisym)
+  by auto
 
 theorem demonic_bottom_top [simp]:
   "demonic \<bottom>  = \<top>"
-  by (simp add: expand_fun_eq inf_fun_eq sup_fun_eq demonic_def simp_set_function inf_bool_eq top_fun_eq bot_fun_eq);
+  by (simp add: expand_fun_eq inf_fun_eq sup_fun_eq demonic_def simp_set_function inf_bool_eq top_fun_eq bot_fun_eq)
 
 theorem demonic_sup_inf:
   "demonic (Q \<squnion> Q') = demonic Q \<sqinter> demonic Q'"
-  by (simp add: expand_fun_eq inf_fun_eq sup_fun_eq demonic_def simp_set_function inf_bool_eq);
+  by (simp add: expand_fun_eq inf_fun_eq sup_fun_eq demonic_def simp_set_function inf_bool_eq)
 
 
 
@@ -106,51 +106,51 @@ such that $Q\ s \ s'$, then the angelic update of $Q$ fails in $s$.
 *}
 
 definition
-  "angelic Q p = {s . (Q s) \<sqinter> p \<noteq> \<bottom>}";
+  "angelic Q p = {s . (Q s) \<sqinter> p \<noteq> \<bottom>}"
 
 lemma mono_angelic[simp]:
-  "mono (angelic R)"; 
-  apply (unfold mono_def);
-  apply (unfold angelic_def);
-  apply auto;
-  apply (erule notE);
-  apply (rule antisym);
-  apply auto;
-  apply (case_tac "R xa \<sqinter> x \<le> R xa \<sqinter> y");
-  apply simp;
-  apply (erule notE);
-  apply (rule_tac inf_greatest);
-  apply auto;
-  apply (rule_tac y = x in order_trans);
-  by auto;
+  "mono (angelic R)" 
+  apply (unfold mono_def)
+  apply (unfold angelic_def)
+  apply auto
+  apply (erule notE)
+  apply (rule antisym)
+  apply auto
+  apply (case_tac "R xa \<sqinter> x \<le> R xa \<sqinter> y")
+  apply simp
+  apply (erule notE)
+  apply (rule_tac inf_greatest)
+  apply auto
+  apply (rule_tac y = x in order_trans)
+  by auto
 
 theorem angelic_bottom [simp]:
-  "angelic R \<bottom>  = {}";
-  by (simp add: angelic_def);
+  "angelic R \<bottom>  = {}"
+  by (simp add: angelic_def)
 
 theorem angelic_disjunctive:
-  "angelic R ((p::'a::boolean_algebra) \<squnion> q) = angelic R p \<squnion> angelic R q";
+  "angelic R ((p::'a::boolean_algebra) \<squnion> q) = angelic R p \<squnion> angelic R q"
 by (simp add: expand_fun_eq inf_fun_eq sup_fun_eq angelic_def simp_set_function inf_bool_eq sup_bool_eq inf_sup_distrib1)
 
 theorem angelic_udisjunctive1:
-  "angelic R ((Sup P)::'a::distributive_complete_lattice) = (SUP p:P . (angelic R p))";
-  apply (simp add: angelic_def);
-  apply (unfold SUPR_def);
-  apply (simp add: inf_sup_distributivity);
-  apply (unfold SUPR_def);
-  apply auto;
-  apply (unfold Sup_bottom);
-  by auto;
+  "angelic R ((Sup P)::'a::distributive_complete_lattice) = (SUP p:P . (angelic R p))"
+  apply (simp add: angelic_def)
+  apply (unfold SUPR_def)
+  apply (simp add: inf_sup_distributivity)
+  apply (unfold SUPR_def)
+  apply auto
+  apply (unfold Sup_bottom)
+  by auto
 
 theorem angelic_udisjunctive:
-  "angelic R ((SUP P)::'a::distributive_complete_lattice) = SUP (\<lambda> w . angelic R (P w))";
-  apply (simp add: angelic_def);
-  apply (unfold SUPR_def);
-  apply (simp add: inf_sup_distributivity);
-  apply (unfold SUPR_def);
-  apply auto;
-  apply (unfold Sup_bottom);
-  by auto;
+  "angelic R ((SUP P)::'a::distributive_complete_lattice) = SUP (\<lambda> w . angelic R (P w))"
+  apply (simp add: angelic_def)
+  apply (unfold SUPR_def)
+  apply (simp add: inf_sup_distributivity)
+  apply (unfold SUPR_def)
+  apply auto
+  apply (unfold Sup_bottom)
+  by auto
 
 
 subsection "The guard of a statement"
@@ -161,22 +161,22 @@ is enabled or fails.
 *}
 
 definition
-  "((grd S)::'a::boolean_algebra) = - (S bot)";
+  "((grd S)::'a::boolean_algebra) = - (S bot)"
 
-lemma grd_choice[simp]: "grd (S \<sqinter> T) = (grd S) \<squnion> (grd T)";
-  by (simp add: grd_def compl_inf inf_fun_eq);
+lemma grd_choice[simp]: "grd (S \<sqinter> T) = (grd S) \<squnion> (grd T)"
+  by (simp add: grd_def compl_inf inf_fun_eq)
 
-lemma grd_demonic: "grd (demonic Q) = {s . \<exists> s' . s' \<in> (Q s) }"; 
-  apply (simp add: grd_def demonic_def);
-  by blast;
+lemma grd_demonic: "grd (demonic Q) = {s . \<exists> s' . s' \<in> (Q s) }" 
+  apply (simp add: grd_def demonic_def)
+  by blast
 
-lemma grd_demonic_2[simp]: "(s \<notin> grd (demonic Q)) = (\<forall> s' . s' \<notin>  (Q s))"; 
-  by (simp add: grd_demonic);
+lemma grd_demonic_2[simp]: "(s \<notin> grd (demonic Q)) = (\<forall> s' . s' \<notin>  (Q s))" 
+  by (simp add: grd_demonic)
 
 
 theorem grd_angelic:
-  "grd (angelic R) = UNIV";
-  by (simp add: grd_def);
+  "grd (angelic R) = UNIV"
+  by (simp add: grd_def)
 
 
-end;
+end
